\question{
    \textbf{Minkowski's inequality :} Let $p\geq 1$ and
    $x=\{x_{i}\}_{1}^{\infty} \in l^p$ and
    $y=\{y_{i}\}_{1}^{\infty} \in l^p$. Then

    \begin{enumerate}
        \item[a.]
              $x+y =
              \{x_{i} + y_{i}\}_{1}^{\infty} \in l^{p}$ and
        \item[b.]
              $(\sum_{1}^{\infty}{|x_{i} + y_{i}|^p})^
              \frac{1}{p}\leq
              (\sum_{1}^{\infty}{|x_{i}|^{p}})^{\frac{1}{p}}
              +
              (\sum_{1}^{\infty}{|y_{i}|^{p}})^{\frac{1}{p}}.$
    \end{enumerate}
}
\begin{proof}
    If $p=1$ then the Minkowski inequality follows from the
    triangle inequality. Let $p>1$ then
    \begin{align}\sum_{1}^{\infty}{\left(|x_{i} + y_{i}|^p\right)}=
    \sum_{1}^{\infty}{\left(|x_i+y_1||x_{i} + y_{i}|^{p-1}\right)}
    &\leq\sum_{1}^{\infty}{\left(|x_i||x_{i} + y_{i}|^{p-1}
    +|y_i||x_{i} + y_{i}|^{p-1}\right)}\\
    &=\sum_{1}^{\infty}{\left(|x_i||x_{i} + y_{i}|^{p-1}\right)}
    +\sum_{1}^{\infty}{\left(|y_i||x_{i} + y_{i}|^{p-1}\right)}
    \label{line2}
    \end{align}
    Now let $q$ be the conjugate exponent of $p$, then we have
    $\frac{1}{p}+\frac{1}{q}=1 \iff p+q=pq \iff p=p(q-1)$. Then,
    from
    \ref{line2}

    $$\left(\sum_{1}^{\infty}{|x_i+y_i|^{(p-1)q}}\right)^{1/q}
    =\left(\sum_{1}^{\infty}{|x_i+y_i|^{p}}\right)^{1/q}
    <\infty$$

    $$\sum_{1}^{\infty}{|x_i||x_{i} + y_{i}|^{p-1}}
    \leq \left(\sum_{1}^{\infty}{|x_i|^p}\right)^{1/p}\cdot
    \left(\sum_{1}^{\infty}{|x_i+y_i|^{(p-1)q}}\right)^{1/q}
    =\left(\sum_{1}^{\infty}{|x_i|^p}\right)^{1/p}\cdot
    \left(\sum_{1}^{\infty}{|x_i+y_i|^{p}}\right)^{1/q}$$
\end{proof}