\question{
    Prove Minkowski's Inequality for Sums.
}

\begin{solution}
    
    \textbf{Minkowski's inequality :} Let $p\geq 1$ and
    $x=\{x_{i}\}_{1}^{\infty} \in l^p$ and
    $y=\{y_{i}\}_{1}^{\infty} \in l^p$. Then

    \begin{enumerate}
        \item[a.]
              $x+y =
              \{x_{i} + y_{i}\}_{1}^{\infty} \in l^{p}$ and
        \item[b.]
        $\left(\sum_{1}^{\infty}{|x_{i} + y_{i}|^p}\right)^
        \frac{1}{p}\leq
        \left(\sum_{1}^{\infty}{|x_{i}|^{p}}\right)^{\frac{1}{p}}
        +
        \left(\sum_{1}^{\infty}{|y_{i}|^{p}}\right)^{\frac{1}{p}}.$
    \end{enumerate}
    First we show that $x+y\in l^p$ by showing that
    $$\left(\sum_{1}^{\infty}{|x_{i} + y_{i}|^p}\right)^{1/p}
    <\infty$$
    We have,
    $$\sum_{1}^{\infty}{|x_{i} + y_{i}|^p}\leq
    \sum_i^{\infty}{\left(|x_i|+|y_i|\right)^p}\leq
    2^{p-1}\left(\sum_i^{\infty}{|x_i|^p}+
    \sum_i^{\infty}{|y_i|^p}\right)<\infty.$$

    Now, since $x,y\in l^p$, $d_p(x,y)<\infty$.
    If $p=1$ then the Minkowski inequality follows from the
    triangle inequality of real numbers. Let $p>1$ then
    \begin{align}\sum_{1}^{\infty}{|x_{i} + y_{i}|^p}=
    \sum_{1}^{\infty}{|x_i+y_1||x_{i} + y_{i}|^{p-1}}
    &\leq\sum_{1}^{\infty}{\left(|x_i||x_{i} + y_{i}|^{p-1}
    +|y_i||x_{i} + y_{i}|^{p-1}\right)}\label{line1}\\
    &=\sum_{1}^{\infty}{\left(|x_i||x_{i} + y_{i}|^{p-1}\right)}
    +\sum_{1}^{\infty}{\left(|y_i||x_{i} + y_{i}|^{p-1}\right)}
    \label{line2}
    \end{align}
    Now let $q$ be the conjugate exponent of $p$, then we have
    $\frac{1}{p}+\frac{1}{q}=1 \iff p+q=pq \iff p=p(q-1)$. Then,
    at line
    \ref{line2}

    $$\left(\sum_{1}^{\infty}{|x_i+y_i|^{(p-1)q}}\right)^{1/q}
    =\left(\sum_{1}^{\infty}{|x_i+y_i|^{p}}\right)^{1/q}
    <\infty$$

    which shows that $\{|x_i+y_i|^{p-1}\}_i^{\infty}\in
    l^q$. Then by Holder's inequality,

    \begin{align}\sum_{1}^{\infty}{|x_i||x_{i} + y_{i}|^{p-1}}
      &\leq \left(\sum_{1}^{\infty}{|x_i|^p}\right)^{1/p}\cdot
      \left(\sum_{1}^{\infty}{|x_i+y_i|^{(p-1)q}}\right)^{1/q}\\
      &=\left(\sum_{1}^{\infty}{|x_i|^p}\right)^{1/p}\cdot
      \left(\sum_{1}^{\infty}{|x_i+y_i|^{p}}\right)^{1/q}
      \label{line4}
    \end{align}

    Using the results from line \ref{line2} and line \ref{line4} on line
    \ref{line1},
    \begin{align}
      \sum_{1}^{\infty}{|x_{i} + y_{i}|^p}
      &\leq \sum_{1}^{\infty}{\left(|x_i||x_{i} + y_{i}|^{p-1}\right)}
      +\sum_{1}^{\infty}{\left(|y_i||x_{i} + y_{i}|^{p-1}\right)}\\
      \text{or,}\hspace*{5mm}
      \sum_{1}^{\infty}{|x_{i} + y_{i}|^p}
      &\leq\left(\sum_{1}^{\infty}{|x_i+y_i|^{p}}\right)^{1/q}
      \cdot\left(\left(\sum_{1}^{\infty}{|x_i|^p}\right)^{1/p}
      +\left(\sum_{1}^{\infty}{|y_i|^p}\right)^{1/p}\right)
    \end{align}
    Dividing both sides by
    $\left(\sum_{1}^{\infty}{|x_i+y_i|^{p}}\right)^{1/q}$,
    we get the Minkowski's inequality (since $1-\frac{1}{q}=\frac{1}{p}$).
    
    \qed
\end{solution}